Wavelet/LTS.lean
@@ -1,0 +1,64 @@
+import Wavelet.Op
+
+namespace Wavelet.LTS
+
+open Op
+
+abbrev LTS (C : Type u) (E : Type v) := C → Trace E → C → Prop
+
+inductive LTS.Plus (R : LTS C E) : LTS C E where
+  | single : R c tr c' → Plus R c tr c'
+  | tail : Plus R c tr c' → R c' tr' c'' → Plus R c (tr ++ tr') c''
+
+inductive LTS.Star (R : LTS C E) : LTS C E where
+  | refl : Star R c .ε c
+  | tail : Star R c tr c' → R c' tr' c'' → Star R c (tr ++ tr') c''
+
+/-- Simulation of two LTS's. -/
+def Simulation
+  (c₁ : C₁) (c₂ : C₂)
+  (R : C₁ → C₂ → Prop)
+  (Step₁ : LTS C₁ E)
+  (Step₂ : LTS C₂ E) :=
+  R c₁ c₂ ∧
+  ∀ c₁ c₂ c₁' tr,
+    R c₁ c₂ →
+    Step₁ c₁ tr c₁' →
+    ∃ c₂',
+      Step₂ c₂ tr c₂' ∧
+      R c₁' c₂'
+
+theorem LTS.step_eq_rhs {R : LTS C E}
+  (h : R c₁ tr c₂)
+  (heq : c₂ = c₂') :
+  R c₁ tr c₂' := by
+  simp [heq] at h
+  exact h
+
+theorem LTS.step_eq_tr_rhs {R : LTS C E}
+  (h : R c₁ tr c₂)
+  (heq₁ : tr = tr')
+  (heq₂ : c₂ = c₂') :
+  R c₁ tr' c₂' := by
+  simp [heq₁, heq₂] at h
+  exact h
+
+theorem LTS.Star.single
+  {R : LTS C E}
+  (h : R c₁ tr c₂) :
+  LTS.Star R c₁ tr c₂ := .tail (.refl) h
+
+theorem LTS.Star.trans
+  {R : LTS C E}
+  {c₁ c₂ c₃ : C}
+  {tr₁ tr₂ : Trace E}
+  (h₁ : LTS.Star R c₁ tr₁ c₂)
+  (h₂ : LTS.Star R c₂ tr₂ c₃) :
+  LTS.Star R c₁ (tr₁ ++ tr₂) c₃ := sorry
+
+theorem LTS.Plus.to_star
+  {R : LTS C E}
+  (h : LTS.Plus R c₁ tr c₂) :
+  LTS.Star R c₁ tr c₂ := sorry
+
+end Wavelet.LTS
